Memory.fst
@@ -2,39 +2,40 @@ module Memory
 
 open Value
 
-type byte = nat
+type address = FStar.UInt64.t
+type byte = FStar.UInt64.t
 
 type memoryState = list (maybeBlinded #byte)
 
-let rec nth (m:list (maybeBlinded #byte)) (n:nat) : maybeBlinded #byte = match m, n with
-  | Nil,     _ -> Blinded 0
-  | hd :: tl, 0 -> hd
-  | hd :: tl, n -> nth tl (n-1)
+let rec nth (m:list (maybeBlinded #byte)) (n:address) : maybeBlinded #byte =
+  match m, n with
+    | Nil,     _   -> Blinded 0uL
+    | hd :: tl, 0uL -> hd
+    | hd :: tl, n   -> nth tl (FStar.UInt64.sub n 1uL)
 
-let _ = assert( forall (m:memoryState) (p:maybeBlinded #byte) (n:nat). nth m n == nth (p :: m) (n+1) )
 
-let equal_memories_have_equal_values (a b: memoryState) (n:nat):
+let equal_memories_have_equal_values (a b: memoryState) (n:address):
     Lemma (requires a = b)
           (ensures (nth a n) = (nth b n))
     = ()
 
-let rec equivalent_memories_have_equivalent_values (a b: memoryState) (n: nat):
+let rec equivalent_memories_have_equivalent_values (a b: memoryState) (n: address):
     Lemma (requires equiv_list a b)
           (ensures equiv (nth a n) (nth b n))
     = match n, a, b  with
-      | 0, _, _ -> ()
-      | _, hl :: tl, hr :: tr -> equivalent_memories_have_equivalent_values tl tr (n - 1)
+      | 0uL, _, _ -> ()
+      | _, hl :: tl, hr :: tr -> equivalent_memories_have_equivalent_values tl tr (FStar.UInt64.sub n 1uL)
       | _ -> ()
 
 
-irreducible let trigger (a b: memoryState) (n:nat) = True
+irreducible let trigger (a b: memoryState) (n:address) = True
 
-let rec equivalent_memories_have_identical_blindedness_somewhere (a b: memoryState) (n:nat):
+let rec equivalent_memories_have_identical_blindedness_somewhere (a b: memoryState) (n:address):
   Lemma (requires equiv_list a b)
         (ensures Blinded? (nth a n) <==> Blinded? (nth b n))
         [SMTPat (trigger a b n)]=
   match n, a, b with
-    | 0, _, _ -> ()
-    | _, hl :: tl, hr :: tr -> equivalent_memories_have_identical_blindedness_somewhere tl tr (n-1)
+    | 0uL, _, _ -> ()
+    | _, hl :: tl, hr :: tr -> equivalent_memories_have_identical_blindedness_somewhere tl tr (FStar.UInt64.sub n 1uL)
     | _ -> ()
 
